\documentclass{article}
\usepackage[utf8]{inputenc}

\title{Proving the Quadratic Formula}
\author{Ethan Xu}
\date{September 2021}

\usepackage{chngcntr}
\usepackage{amssymb}
\usepackage{ragged2e}
\usepackage{amsmath,amsthm}

\renewcommand{\qed}{\hfill\square}

\counterwithin*{equation}{section}
\counterwithin*{equation}{subsection}


\begin{document}

\maketitle

\section{Introduction}

The quadratic formula states that:

\begin{equation}
    x=\frac{-b\pm\sqrt{b^2-4ac}}{2a}
\end{equation}

when given a quadratic equation such as:

\begin{equation}
    ax^2+bx+c=0
\end{equation}

\section{Proof}

\begin{equation}
    ax^2+bx+c=0
\end{equation}

\begin{equation}
    ax^2+bx=-c
\end{equation}

\begin{equation}
    x^2+\frac{b}{a}x=-\frac{c}{a}
\end{equation}

\begin{equation}
    x^2+\frac{b}{a}x+\frac{b^2}{4a^2}=-\frac{c}{a}+\frac{b^2}{4a^2}
\end{equation}

\begin{equation}
    (x+\frac{b}{2a})^2=-\frac{c}{a}+\frac{b^2}{4a^2}
\end{equation}

\begin{equation}
    x+\frac{b}{2a}=\pm\sqrt{-\frac{c}{a}+\frac{b^2}{4a^2}}
\end{equation}

\begin{equation}
    x=-\frac{b}{2a}\pm\sqrt{-\frac{c}{a}+\frac{b^2}{4a^2}}
\end{equation}

\begin{equation}
    x=-\frac{b}{2a}\pm\frac{\sqrt{-\frac{c}{a}\cdot(2a)^2+\frac{b^2}{4a^2}\cdot(2a)^2}}{2a}
\end{equation}

\begin{equation}
    x=-\frac{b}{2a}\pm\frac{\sqrt{-4ac+b^2}}{2a}
\end{equation}

\begin{equation}
    x=\frac{-b\pm\sqrt{b^2-4ac}}{2a}
\end{equation}

$\qed$

\end{document}

